src/tls/TLSConstants.fst
@@ -244,34 +244,34 @@ let is_handshake13_signatureScheme = function
 
 val signatureSchemeBytes: s:signatureScheme -> lbytes 2
 let signatureSchemeBytes = function
-  | RSA_PKCS1_SHA256       -> abyte2 (0x04z, 0x01z)
-  | RSA_PKCS1_SHA384       -> abyte2 (0x05z, 0x01z)
-  | RSA_PKCS1_SHA512       -> abyte2 (0x06z, 0x01z)
-  | ECDSA_SECP256R1_SHA256 -> abyte2 (0x04z, 0x03z)
-  | ECDSA_SECP384R1_SHA384 -> abyte2 (0x05z, 0x03z)
-  | ECDSA_SECP521R1_SHA512 -> abyte2 (0x06z, 0x03z)
-  | RSA_PSS_SHA256         -> abyte2 (0x08z, 0x04z)
-  | RSA_PSS_SHA384         -> abyte2 (0x08z, 0x05z)
-  | RSA_PSS_SHA512         -> abyte2 (0x08z, 0x06z)
-  //| ED25519_SHA512         -> abyte2 (0x08z, 0x07z)
-  //| ED448_SHAKE256         -> abyte2 (0x08z, 0x08z)
-  | RSA_PKCS1_SHA1         -> abyte2 (0x02z, 0x01z)
-  | RSA_PKCS1_MD5SHA1      -> abyte2 (0xFFz, 0xFFz)
-  | ECDSA_SHA1             -> abyte2 (0x02z, 0x03z)
-  | DSA_SHA1               -> abyte2 (0x02z, 0x02z)
-  | DSA_SHA256             -> abyte2 (0x04z, 0x02z)
-  | DSA_SHA384             -> abyte2 (0x05z, 0x02z)
-  | DSA_SHA512             -> abyte2 (0x06z, 0x02z)
+  | RSA_PKCS1_SHA256       -> twobytes (0x04z, 0x01z)
+  | RSA_PKCS1_SHA384       -> twobytes (0x05z, 0x01z)
+  | RSA_PKCS1_SHA512       -> twobytes (0x06z, 0x01z)
+  | ECDSA_SECP256R1_SHA256 -> twobytes (0x04z, 0x03z)
+  | ECDSA_SECP384R1_SHA384 -> twobytes (0x05z, 0x03z)
+  | ECDSA_SECP521R1_SHA512 -> twobytes (0x06z, 0x03z)
+  | RSA_PSS_SHA256         -> twobytes (0x08z, 0x04z)
+  | RSA_PSS_SHA384         -> twobytes (0x08z, 0x05z)
+  | RSA_PSS_SHA512         -> twobytes (0x08z, 0x06z)
+  //| ED25519_SHA512         -> twobytes (0x08z, 0x07z)
+  //| ED448_SHAKE256         -> twobytes (0x08z, 0x08z)
+  | RSA_PKCS1_SHA1         -> twobytes (0x02z, 0x01z)
+  | RSA_PKCS1_MD5SHA1      -> twobytes (0xFFz, 0xFFz)
+  | ECDSA_SHA1             -> twobytes (0x02z, 0x03z)
+  | DSA_SHA1               -> twobytes (0x02z, 0x02z)
+  | DSA_SHA256             -> twobytes (0x04z, 0x02z)
+  | DSA_SHA384             -> twobytes (0x05z, 0x02z)
+  | DSA_SHA512             -> twobytes (0x06z, 0x02z)
   | SIG_UNKNOWN codepoint  -> codepoint
 
 let signatureSchemeBytes_is_injective
   (s1 s2: signatureScheme)
 : Lemma
-  (requires (Seq.equal (signatureSchemeBytes s1) (signatureSchemeBytes s2)))
+  (requires (signatureSchemeBytes s1 == signatureSchemeBytes s2))
   (ensures (s1 == s2))
 = if (SIG_UNKNOWN? s1) = (SIG_UNKNOWN? s2)
   then ()
-  else assume (s1 == s2) // TODO: strengthen int_of_bytes vs. abyte2
+  else assume (s1 == s2) // TODO: strengthen int_of_bytes vs. twobytes
 
 val parseSignatureScheme: pinverse_t signatureSchemeBytes
 let parseSignatureScheme b =
@@ -354,7 +354,8 @@ let signatureScheme_of_sigHashAlg sa ha =
   | (DSA,    Hash SHA512) -> DSA_SHA512
   | (RSASIG, MD5SHA1)     -> RSA_PKCS1_MD5SHA1
   | _ -> // Map everything else to OBSOLETE 0x0000
-    lemma_repr_bytes_values 0x0000; int_of_bytes_of_int 2 0x0000;
+    lemma_repr_bytes_values 0x0000;
+    int_of_bytes_of_int #2 0x0000;
     SIG_UNKNOWN (bytes_of_int 2 0)
 
 (** Encryption key sizes *)
@@ -447,9 +448,9 @@ let compressionBytes comp =
 
 (** Parsing function for compression algorithm *)
 val parseCompression: b:lbytes 1
-  -> Tot (cm:compression{Seq.equal (compressionBytes cm) b})
+  -> Tot (cm:compression{compressionBytes cm == b})
 let parseCompression b =
-  match cbyte b with
+  match b.[0ul] with
   | 0z -> NullCompression
   | b  -> UnknownCompression b
 
@@ -462,7 +463,7 @@ val parseCompressions: b:bytes -> Tot (list compression) (decreases (length b))
 let rec parseCompressions b =
   if length b > 0
   then
-    let cmB,b = split b 1 in
+    let cmB,b = split b 1ul in
     let cm = parseCompression cmB in
     cm::(parseCompressions b)
   else []
@@ -485,12 +486,12 @@ let rec compressionMethodsBytes cms =
 val versionBytes: protocolVersion' -> Tot (lbytes 2)
 let versionBytes pv =
   match pv with
-  | SSL_3p0 -> abyte2 ( 3z, 0z)
-  | TLS_1p0 -> abyte2 ( 3z, 1z)
-  | TLS_1p1 -> abyte2 ( 3z, 2z )
-  | TLS_1p2 -> abyte2 ( 3z, 3z )
-  | TLS_1p3 -> abyte2 ( 3z, 4z )
-  | UnknownVersion a b -> abyte2 ( a, b )
+  | SSL_3p0 -> twobytes ( 3z, 0z)
+  | TLS_1p0 -> twobytes ( 3z, 1z)
+  | TLS_1p1 -> twobytes ( 3z, 2z )
+  | TLS_1p2 -> twobytes ( 3z, 3z )
+  | TLS_1p3 -> twobytes ( 3z, 4z )
+  | UnknownVersion a b -> twobytes ( a, b )
 
 (** Parsing function for the protocol version *)
 val parseVersion: pinverse_t versionBytes
@@ -511,7 +512,7 @@ let inverse_version x = ()
 
 val pinverse_version: x:_ -> Lemma
   (requires True)
-  (ensures (lemma_pinverse_f_g Seq.equal versionBytes parseVersion x))
+  (ensures (lemma_pinverse_f_g Bytes.equal versionBytes parseVersion x))
   [SMTPat (versionBytes (Correct?._0 (parseVersion x)))]
 let pinverse_version x = ()
 
@@ -520,7 +521,7 @@ let pinverse_version x = ()
 // https://tlswg.github.io/tls13-spec/#rfc.section.4.2.1
 let draft = 21z
 let versionBytes_draft: protocolVersion -> Tot (lbytes 2) = function
-  | TLS_1p3 -> abyte2 ( 127z, draft )
+  | TLS_1p3 -> twobytes ( 127z, draft )
   | pv -> versionBytes pv
 val parseVersion_draft: pinverse_t versionBytes_draft
 let parseVersion_draft v =
@@ -553,7 +554,7 @@ let string_of_pv = function
   | TLS_1p1 -> "1.1"
   | TLS_1p2 -> "1.2"
   | TLS_1p3 -> "1.3"
-  | UnknownVersion a b -> "Unknown protocol version: " ^ (print_bytes (abyte2 (a, b)))
+  | UnknownVersion a b -> "Unknown protocol version: " ^ (print_bytes (twobytes (a, b)))
 
 (* JK: injectivity proof requires extra specification for the UnknownCipherSuite objects as they
    have to be distinct from the 'correct' ones *)
@@ -561,108 +562,108 @@ val cipherSuiteBytesOpt: cipherSuite -> Tot (option (lbytes 2))
 let cipherSuiteBytesOpt cs =
   let open CoreCrypto in
   let open Hashing.Spec in
-  let abyte2 b: option (lbytes 2) = Some (abyte2 b) in
+  let twobytes b: option (lbytes 2) = Some (twobytes b) in
     match cs with
-    | UnknownCipherSuite b1 b2 -> abyte2 (b1,b2)
-    | NullCipherSuite                                              -> abyte2 ( 0x00z, 0x00z )
+    | UnknownCipherSuite b1 b2 -> twobytes (b1,b2)
+    | NullCipherSuite                                              -> twobytes ( 0x00z, 0x00z )
 
-    | CipherSuite13 AES_128_GCM       SHA256                       -> abyte2 ( 0x13z, 0x01z )
-    | CipherSuite13 AES_256_GCM       SHA384                       -> abyte2 ( 0x13z, 0x02z )
-    | CipherSuite13 CHACHA20_POLY1305 SHA256                       -> abyte2 ( 0x13z, 0x03z )
-    | CipherSuite13 AES_128_CCM       SHA256                       -> abyte2 ( 0x13z, 0x04z )
-    | CipherSuite13 AES_128_CCM_8     SHA256                       -> abyte2 ( 0x13z, 0x05z )
+    | CipherSuite13 AES_128_GCM       SHA256                       -> twobytes ( 0x13z, 0x01z )
+    | CipherSuite13 AES_256_GCM       SHA384                       -> twobytes ( 0x13z, 0x02z )
+    | CipherSuite13 CHACHA20_POLY1305 SHA256                       -> twobytes ( 0x13z, 0x03z )
+    | CipherSuite13 AES_128_CCM       SHA256                       -> twobytes ( 0x13z, 0x04z )
+    | CipherSuite13 AES_128_CCM_8     SHA256                       -> twobytes ( 0x13z, 0x05z )
 
-    | CipherSuite Kex_RSA None (MACOnly MD5)                       -> abyte2 ( 0x00z, 0x01z )
-    | CipherSuite Kex_RSA None (MACOnly SHA1)                      -> abyte2 ( 0x00z, 0x02z )
-    | CipherSuite Kex_RSA None (MACOnly SHA256)                    -> abyte2 ( 0x00z, 0x3Bz )
-    | CipherSuite Kex_RSA None(MtE (Stream RC4_128) MD5)           -> abyte2 ( 0x00z, 0x04z )
-    | CipherSuite Kex_RSA None(MtE (Stream RC4_128) SHA1)          -> abyte2 ( 0x00z, 0x05z )
+    | CipherSuite Kex_RSA None (MACOnly MD5)                       -> twobytes ( 0x00z, 0x01z )
+    | CipherSuite Kex_RSA None (MACOnly SHA1)                      -> twobytes ( 0x00z, 0x02z )
+    | CipherSuite Kex_RSA None (MACOnly SHA256)                    -> twobytes ( 0x00z, 0x3Bz )
+    | CipherSuite Kex_RSA None(MtE (Stream RC4_128) MD5)           -> twobytes ( 0x00z, 0x04z )
+    | CipherSuite Kex_RSA None(MtE (Stream RC4_128) SHA1)          -> twobytes ( 0x00z, 0x05z )
 
-    | CipherSuite Kex_RSA None(MtE (Block TDES_EDE_CBC) SHA1)      -> abyte2 ( 0x00z, 0x0Az )
-    | CipherSuite Kex_RSA None(MtE (Block AES_128_CBC) SHA1)       -> abyte2 ( 0x00z, 0x2Fz )
-    | CipherSuite Kex_RSA None(MtE (Block AES_256_CBC) SHA1)       -> abyte2 ( 0x00z, 0x35z )
-    | CipherSuite Kex_RSA None(MtE (Block AES_128_CBC) SHA256)     -> abyte2 ( 0x00z, 0x3Cz )
-    | CipherSuite Kex_RSA None(MtE (Block AES_256_CBC) SHA256)     -> abyte2 ( 0x00z, 0x3Dz )
-
-    (**************************************************************************)
-    | CipherSuite Kex_DH (Some DSA)     (MtE (Block TDES_EDE_CBC) SHA1)   -> abyte2 ( 0x00z, 0x0Dz )
-    | CipherSuite Kex_DH (Some RSASIG)  (MtE (Block TDES_EDE_CBC) SHA1)   -> abyte2 ( 0x00z, 0x10z )
-    | CipherSuite Kex_DHE (Some DSA)    (MtE (Block TDES_EDE_CBC) SHA1)   -> abyte2 ( 0x00z, 0x13z )
-    | CipherSuite Kex_DHE (Some RSASIG) (MtE (Block TDES_EDE_CBC) SHA1)   -> abyte2 ( 0x00z, 0x16z )
-
-    | CipherSuite Kex_DH (Some DSA)     (MtE (Block AES_128_CBC) SHA1)    -> abyte2 ( 0x00z, 0x30z )
-    | CipherSuite Kex_DH (Some RSASIG)  (MtE (Block AES_128_CBC) SHA1)    -> abyte2 ( 0x00z, 0x31z )
-    | CipherSuite Kex_DHE (Some DSA)    (MtE (Block AES_128_CBC) SHA1)    -> abyte2 ( 0x00z, 0x32z )
-    | CipherSuite Kex_DHE (Some RSASIG) (MtE (Block AES_128_CBC) SHA1)    -> abyte2 ( 0x00z, 0x33z )
-
-    | CipherSuite Kex_DH (Some DSA)     (MtE (Block AES_256_CBC) SHA1)    -> abyte2 ( 0x00z, 0x36z )
-    | CipherSuite Kex_DH (Some RSASIG)  (MtE (Block AES_256_CBC) SHA1)    -> abyte2 ( 0x00z, 0x37z )
-    | CipherSuite Kex_DHE (Some DSA)    (MtE (Block AES_256_CBC) SHA1)    -> abyte2 ( 0x00z, 0x38z )
-    | CipherSuite Kex_DHE (Some RSASIG) (MtE (Block AES_256_CBC) SHA1)    -> abyte2 ( 0x00z, 0x39z )
-
-    | CipherSuite Kex_DH (Some DSA)     (MtE (Block AES_128_CBC) SHA256)  -> abyte2 ( 0x00z, 0x3Ez )
-    | CipherSuite Kex_DH (Some RSASIG)  (MtE (Block AES_128_CBC) SHA256)  -> abyte2 ( 0x00z, 0x3Fz )
-    | CipherSuite Kex_DHE (Some DSA)    (MtE (Block AES_128_CBC) SHA256)  -> abyte2 ( 0x00z, 0x40z )
-    | CipherSuite Kex_DHE (Some RSASIG) (MtE (Block AES_128_CBC) SHA256)  -> abyte2 ( 0x00z, 0x67z )
-
-    | CipherSuite Kex_DH (Some DSA)     (MtE (Block AES_256_CBC) SHA256)  -> abyte2 ( 0x00z, 0x68z )
-    | CipherSuite Kex_DH (Some RSASIG)  (MtE (Block AES_256_CBC) SHA256)  -> abyte2 ( 0x00z, 0x69z )
-    | CipherSuite Kex_DHE (Some DSA)    (MtE (Block AES_256_CBC) SHA256)  -> abyte2 ( 0x00z, 0x6Az )
-    | CipherSuite Kex_DHE (Some RSASIG) (MtE (Block AES_256_CBC) SHA256)  -> abyte2 ( 0x00z, 0x6Bz )
+    | CipherSuite Kex_RSA None(MtE (Block TDES_EDE_CBC) SHA1)      -> twobytes ( 0x00z, 0x0Az )
+    | CipherSuite Kex_RSA None(MtE (Block AES_128_CBC) SHA1)       -> twobytes ( 0x00z, 0x2Fz )
+    | CipherSuite Kex_RSA None(MtE (Block AES_256_CBC) SHA1)       -> twobytes ( 0x00z, 0x35z )
+    | CipherSuite Kex_RSA None(MtE (Block AES_128_CBC) SHA256)     -> twobytes ( 0x00z, 0x3Cz )
+    | CipherSuite Kex_RSA None(MtE (Block AES_256_CBC) SHA256)     -> twobytes ( 0x00z, 0x3Dz )
 
     (**************************************************************************)
-    | CipherSuite Kex_ECDHE (Some RSASIG) (MtE (Stream RC4_128) SHA1)       -> abyte2 ( 0xc0z, 0x11z )
-    | CipherSuite Kex_ECDHE (Some RSASIG) (MtE (Block TDES_EDE_CBC) SHA1)   -> abyte2 ( 0xc0z, 0x12z )
-    | CipherSuite Kex_ECDHE (Some RSASIG) (MtE (Block AES_128_CBC) SHA1)    -> abyte2 ( 0xc0z, 0x13z )
-    | CipherSuite Kex_ECDHE (Some RSASIG) (MtE (Block AES_256_CBC) SHA1)    -> abyte2 ( 0xc0z, 0x14z )
-    | CipherSuite Kex_ECDHE (Some RSASIG) (MtE (Block AES_128_CBC) SHA256)  -> abyte2 ( 0xc0z, 0x27z )
-    | CipherSuite Kex_ECDHE (Some RSASIG) (MtE (Block AES_256_CBC) SHA384)  -> abyte2 ( 0xc0z, 0x28z )
+    | CipherSuite Kex_DH (Some DSA)     (MtE (Block TDES_EDE_CBC) SHA1)   -> twobytes ( 0x00z, 0x0Dz )
+    | CipherSuite Kex_DH (Some RSASIG)  (MtE (Block TDES_EDE_CBC) SHA1)   -> twobytes ( 0x00z, 0x10z )
+    | CipherSuite Kex_DHE (Some DSA)    (MtE (Block TDES_EDE_CBC) SHA1)   -> twobytes ( 0x00z, 0x13z )
+    | CipherSuite Kex_DHE (Some RSASIG) (MtE (Block TDES_EDE_CBC) SHA1)   -> twobytes ( 0x00z, 0x16z )
 
-    | CipherSuite Kex_ECDHE (Some RSASIG) (AEAD AES_128_GCM SHA256) -> abyte2 ( 0xc0z, 0x2fz )
-    | CipherSuite Kex_ECDHE (Some ECDSA)  (AEAD AES_128_GCM SHA256) -> abyte2 ( 0xc0z, 0x2bz )
-    | CipherSuite Kex_ECDHE (Some RSASIG) (AEAD AES_256_GCM SHA384) -> abyte2 ( 0xc0z, 0x30z )
-    | CipherSuite Kex_ECDHE (Some ECDSA) (AEAD AES_256_GCM SHA384) -> abyte2 ( 0xc0z, 0x2cz )
+    | CipherSuite Kex_DH (Some DSA)     (MtE (Block AES_128_CBC) SHA1)    -> twobytes ( 0x00z, 0x30z )
+    | CipherSuite Kex_DH (Some RSASIG)  (MtE (Block AES_128_CBC) SHA1)    -> twobytes ( 0x00z, 0x31z )
+    | CipherSuite Kex_DHE (Some DSA)    (MtE (Block AES_128_CBC) SHA1)    -> twobytes ( 0x00z, 0x32z )
+    | CipherSuite Kex_DHE (Some RSASIG) (MtE (Block AES_128_CBC) SHA1)    -> twobytes ( 0x00z, 0x33z )
 
-    (**************************************************************************)
-    | CipherSuite Kex_PSK_DHE None (AEAD AES_128_GCM SHA256) -> abyte2 ( 0x00z, 0xaaz )
-    | CipherSuite Kex_PSK_DHE None (AEAD AES_256_GCM SHA384) -> abyte2 ( 0x00z, 0xabz )
-    | CipherSuite Kex_PSK_ECDHE None (AEAD AES_128_GCM SHA256) -> abyte2 ( 0xd0z, 0x01z )
-    | CipherSuite Kex_PSK_ECDHE None (AEAD AES_256_GCM SHA384) -> abyte2 ( 0xd0z, 0x02z )
+    | CipherSuite Kex_DH (Some DSA)     (MtE (Block AES_256_CBC) SHA1)    -> twobytes ( 0x00z, 0x36z )
+    | CipherSuite Kex_DH (Some RSASIG)  (MtE (Block AES_256_CBC) SHA1)    -> twobytes ( 0x00z, 0x37z )
+    | CipherSuite Kex_DHE (Some DSA)    (MtE (Block AES_256_CBC) SHA1)    -> twobytes ( 0x00z, 0x38z )
+    | CipherSuite Kex_DHE (Some RSASIG) (MtE (Block AES_256_CBC) SHA1)    -> twobytes ( 0x00z, 0x39z )
 
-    (**************************************************************************)
-    | CipherSuite Kex_DHE None   (MtE (Stream RC4_128) MD5)         -> abyte2 ( 0x00z, 0x18z )
-    | CipherSuite Kex_DHE None   (MtE (Block TDES_EDE_CBC) SHA1)    -> abyte2 ( 0x00z, 0x1Bz )
-    | CipherSuite Kex_DHE None   (MtE (Block AES_128_CBC) SHA1)     -> abyte2 ( 0x00z, 0x34z )
-    | CipherSuite Kex_DHE None   (MtE (Block AES_256_CBC) SHA1)     -> abyte2 ( 0x00z, 0x3Az )
-    | CipherSuite Kex_DHE None   (MtE (Block AES_128_CBC) SHA256)   -> abyte2 ( 0x00z, 0x6Cz )
-    | CipherSuite Kex_DHE None   (MtE (Block AES_256_CBC) SHA256)   -> abyte2 ( 0x00z, 0x6Dz )
+    | CipherSuite Kex_DH (Some DSA)     (MtE (Block AES_128_CBC) SHA256)  -> twobytes ( 0x00z, 0x3Ez )
+    | CipherSuite Kex_DH (Some RSASIG)  (MtE (Block AES_128_CBC) SHA256)  -> twobytes ( 0x00z, 0x3Fz )
+    | CipherSuite Kex_DHE (Some DSA)    (MtE (Block AES_128_CBC) SHA256)  -> twobytes ( 0x00z, 0x40z )
+    | CipherSuite Kex_DHE (Some RSASIG) (MtE (Block AES_128_CBC) SHA256)  -> twobytes ( 0x00z, 0x67z )
 
-    (**************************************************************************)
-    | CipherSuite Kex_RSA None     (AEAD AES_128_GCM SHA256) -> abyte2( 0x00z, 0x9Cz )
-    | CipherSuite Kex_RSA None     (AEAD AES_256_GCM SHA384) -> abyte2( 0x00z, 0x9Dz )
-
-    | CipherSuite Kex_DHE (Some RSASIG) (AEAD AES_128_GCM SHA256) -> abyte2( 0x00z, 0x9Ez )
-    | CipherSuite Kex_DHE (Some RSASIG) (AEAD AES_256_GCM SHA384) -> abyte2( 0x00z, 0x9Fz )
-    | CipherSuite Kex_DH (Some RSASIG)  (AEAD AES_128_GCM SHA256) -> abyte2( 0x00z, 0xA0z )
-    | CipherSuite Kex_DH (Some RSASIG)  (AEAD AES_256_GCM SHA384) -> abyte2( 0x00z, 0xA1z )
-
-    | CipherSuite Kex_DHE (Some DSA) (AEAD AES_128_GCM SHA256) -> abyte2( 0x00z, 0xA2z )
-    | CipherSuite Kex_DHE (Some DSA) (AEAD AES_256_GCM SHA384) -> abyte2( 0x00z, 0xA3z )
-    | CipherSuite Kex_DH (Some DSA)  (AEAD AES_128_GCM SHA256) -> abyte2( 0x00z, 0xA4z )
-    | CipherSuite Kex_DH (Some DSA)  (AEAD AES_256_GCM SHA384) -> abyte2( 0x00z, 0xA5z )
-
-    | CipherSuite Kex_DHE None (AEAD AES_128_GCM SHA256) -> abyte2( 0x00z, 0xA6z )
-    | CipherSuite Kex_DHE None (AEAD AES_256_GCM SHA384) -> abyte2( 0x00z, 0xA7z )
+    | CipherSuite Kex_DH (Some DSA)     (MtE (Block AES_256_CBC) SHA256)  -> twobytes ( 0x00z, 0x68z )
+    | CipherSuite Kex_DH (Some RSASIG)  (MtE (Block AES_256_CBC) SHA256)  -> twobytes ( 0x00z, 0x69z )
+    | CipherSuite Kex_DHE (Some DSA)    (MtE (Block AES_256_CBC) SHA256)  -> twobytes ( 0x00z, 0x6Az )
+    | CipherSuite Kex_DHE (Some RSASIG) (MtE (Block AES_256_CBC) SHA256)  -> twobytes ( 0x00z, 0x6Bz )
 
     (**************************************************************************)
-    | CipherSuite Kex_ECDHE (Some RSASIG) (AEAD CHACHA20_POLY1305 SHA256) -> abyte2( 0xccz, 0xa8z )
-    | CipherSuite Kex_ECDHE (Some ECDSA) (AEAD CHACHA20_POLY1305 SHA256)  -> abyte2( 0xccz, 0xa9z )
-    | CipherSuite Kex_DHE (Some RSASIG) (AEAD CHACHA20_POLY1305 SHA256)   -> abyte2( 0xccz, 0xaaz )
-    | CipherSuite Kex_PSK None (AEAD CHACHA20_POLY1305 SHA256)            -> abyte2( 0xccz, 0xabz )
-    | CipherSuite Kex_PSK_ECDHE None (AEAD CHACHA20_POLY1305 SHA256)      -> abyte2( 0xccz, 0xacz )
-    | CipherSuite Kex_PSK_DHE None (AEAD CHACHA20_POLY1305 SHA256)        -> abyte2( 0xccz, 0xadz )
+    | CipherSuite Kex_ECDHE (Some RSASIG) (MtE (Stream RC4_128) SHA1)       -> twobytes ( 0xc0z, 0x11z )
+    | CipherSuite Kex_ECDHE (Some RSASIG) (MtE (Block TDES_EDE_CBC) SHA1)   -> twobytes ( 0xc0z, 0x12z )
+    | CipherSuite Kex_ECDHE (Some RSASIG) (MtE (Block AES_128_CBC) SHA1)    -> twobytes ( 0xc0z, 0x13z )
+    | CipherSuite Kex_ECDHE (Some RSASIG) (MtE (Block AES_256_CBC) SHA1)    -> twobytes ( 0xc0z, 0x14z )
+    | CipherSuite Kex_ECDHE (Some RSASIG) (MtE (Block AES_128_CBC) SHA256)  -> twobytes ( 0xc0z, 0x27z )
+    | CipherSuite Kex_ECDHE (Some RSASIG) (MtE (Block AES_256_CBC) SHA384)  -> twobytes ( 0xc0z, 0x28z )
 
-    | SCSV (TLS_EMPTY_RENEGOTIATION_INFO_SCSV)         -> abyte2 ( 0x00z, 0xFFz )
+    | CipherSuite Kex_ECDHE (Some RSASIG) (AEAD AES_128_GCM SHA256) -> twobytes ( 0xc0z, 0x2fz )
+    | CipherSuite Kex_ECDHE (Some ECDSA)  (AEAD AES_128_GCM SHA256) -> twobytes ( 0xc0z, 0x2bz )
+    | CipherSuite Kex_ECDHE (Some RSASIG) (AEAD AES_256_GCM SHA384) -> twobytes ( 0xc0z, 0x30z )
+    | CipherSuite Kex_ECDHE (Some ECDSA) (AEAD AES_256_GCM SHA384) -> twobytes ( 0xc0z, 0x2cz )
+
+    (**************************************************************************)
+    | CipherSuite Kex_PSK_DHE None (AEAD AES_128_GCM SHA256) -> twobytes ( 0x00z, 0xaaz )
+    | CipherSuite Kex_PSK_DHE None (AEAD AES_256_GCM SHA384) -> twobytes ( 0x00z, 0xabz )
+    | CipherSuite Kex_PSK_ECDHE None (AEAD AES_128_GCM SHA256) -> twobytes ( 0xd0z, 0x01z )
+    | CipherSuite Kex_PSK_ECDHE None (AEAD AES_256_GCM SHA384) -> twobytes ( 0xd0z, 0x02z )
+
+    (**************************************************************************)
+    | CipherSuite Kex_DHE None   (MtE (Stream RC4_128) MD5)         -> twobytes ( 0x00z, 0x18z )
+    | CipherSuite Kex_DHE None   (MtE (Block TDES_EDE_CBC) SHA1)    -> twobytes ( 0x00z, 0x1Bz )
+    | CipherSuite Kex_DHE None   (MtE (Block AES_128_CBC) SHA1)     -> twobytes ( 0x00z, 0x34z )
+    | CipherSuite Kex_DHE None   (MtE (Block AES_256_CBC) SHA1)     -> twobytes ( 0x00z, 0x3Az )
+    | CipherSuite Kex_DHE None   (MtE (Block AES_128_CBC) SHA256)   -> twobytes ( 0x00z, 0x6Cz )
+    | CipherSuite Kex_DHE None   (MtE (Block AES_256_CBC) SHA256)   -> twobytes ( 0x00z, 0x6Dz )
+
+    (**************************************************************************)
+    | CipherSuite Kex_RSA None     (AEAD AES_128_GCM SHA256) -> twobytes( 0x00z, 0x9Cz )
+    | CipherSuite Kex_RSA None     (AEAD AES_256_GCM SHA384) -> twobytes( 0x00z, 0x9Dz )
+
+    | CipherSuite Kex_DHE (Some RSASIG) (AEAD AES_128_GCM SHA256) -> twobytes( 0x00z, 0x9Ez )
+    | CipherSuite Kex_DHE (Some RSASIG) (AEAD AES_256_GCM SHA384) -> twobytes( 0x00z, 0x9Fz )
+    | CipherSuite Kex_DH (Some RSASIG)  (AEAD AES_128_GCM SHA256) -> twobytes( 0x00z, 0xA0z )
+    | CipherSuite Kex_DH (Some RSASIG)  (AEAD AES_256_GCM SHA384) -> twobytes( 0x00z, 0xA1z )
+
+    | CipherSuite Kex_DHE (Some DSA) (AEAD AES_128_GCM SHA256) -> twobytes( 0x00z, 0xA2z )
+    | CipherSuite Kex_DHE (Some DSA) (AEAD AES_256_GCM SHA384) -> twobytes( 0x00z, 0xA3z )
+    | CipherSuite Kex_DH (Some DSA)  (AEAD AES_128_GCM SHA256) -> twobytes( 0x00z, 0xA4z )
+    | CipherSuite Kex_DH (Some DSA)  (AEAD AES_256_GCM SHA384) -> twobytes( 0x00z, 0xA5z )
+
+    | CipherSuite Kex_DHE None (AEAD AES_128_GCM SHA256) -> twobytes( 0x00z, 0xA6z )
+    | CipherSuite Kex_DHE None (AEAD AES_256_GCM SHA384) -> twobytes( 0x00z, 0xA7z )
+
+    (**************************************************************************)
+    | CipherSuite Kex_ECDHE (Some RSASIG) (AEAD CHACHA20_POLY1305 SHA256) -> twobytes( 0xccz, 0xa8z )
+    | CipherSuite Kex_ECDHE (Some ECDSA) (AEAD CHACHA20_POLY1305 SHA256)  -> twobytes( 0xccz, 0xa9z )
+    | CipherSuite Kex_DHE (Some RSASIG) (AEAD CHACHA20_POLY1305 SHA256)   -> twobytes( 0xccz, 0xaaz )
+    | CipherSuite Kex_PSK None (AEAD CHACHA20_POLY1305 SHA256)            -> twobytes( 0xccz, 0xabz )
+    | CipherSuite Kex_PSK_ECDHE None (AEAD CHACHA20_POLY1305 SHA256)      -> twobytes( 0xccz, 0xacz )
+    | CipherSuite Kex_PSK_DHE None (AEAD CHACHA20_POLY1305 SHA256)        -> twobytes( 0xccz, 0xadz )
+
+    | SCSV (TLS_EMPTY_RENEGOTIATION_INFO_SCSV)         -> twobytes ( 0x00z, 0xFFz )
     | _ -> None
 
 let validCipherSuite (c:cipherSuite) = Some? (cipherSuiteBytesOpt c)
@@ -815,7 +816,7 @@ val pinverse_cipherSuite : x:lbytes 2 -> Lemma
 	    (Correct? y ==>
               (if UnknownCipherSuite? (Correct?._0 y) then true
               else Some? (cipherSuiteBytesOpt (Correct?._0 y))
-               /\ Seq.equal x (Some?.v (cipherSuiteBytesOpt (Correct?._0 y)))))))
+               /\ Bytes.equal x (Some?.v (cipherSuiteBytesOpt (Correct?._0 y)))))))
   [SMTPat (cipherSuiteBytesOpt (Correct?._0 (parseCipherSuiteAux x)))]
 let pinverse_cipherSuite x = ()
 
@@ -837,7 +838,7 @@ let rec cipherSuitesBytes css =
 val parseCipherSuites: b:bytes -> Tot (result (list (c:cipherSuite{validCipherSuite c}))) (decreases (length b))
 let rec parseCipherSuites b =
   if length b > 1 then
-    let (b0,b1) = split b 2 in
+    let (b0,b1) = split b 2ul in
     match parseCipherSuites b1 with
       | Correct(css) ->
 	(match parseCipherSuite b0 with
@@ -863,8 +864,8 @@ let rec inverse_cipherSuites x =
   | cs::css ->
      assume (~ (UnknownCipherSuite? cs)); // TODO enforce it
      let b = (cipherSuiteBytes cs) @| (cipherSuitesBytes css) in
-     let (b0,b1) = split b 2 in
-     lemma_append_inj b0 b1 (cipherSuiteBytes cs) (cipherSuitesBytes css);
+     let (b0,b1) = split b 2ul in
+     //lemma_append_inj b0 b1 (cipherSuiteBytes cs) (cipherSuitesBytes css); //TODO bytes NS 09/27
      inverse_cipherSuite cs;
      inverse_cipherSuites css
 
@@ -938,9 +939,9 @@ let sigAlg_of_ciphersuite cs =
 type prflabel = bytes
 
 (** Key schedule labels *)
-let extract_label          = utf8 "master secret"
-let extended_extract_label = utf8 "extended master secret"
-let kdf_label              = utf8 "key expansion"
+let extract_label          = utf8_encode "master secret"
+let extended_extract_label = utf8_encode "extended master secret"
+let kdf_label              = utf8_encode "key expansion"
 
 (** PRF definitions based on the protocol version *)
 type prePrfAlg =
@@ -1338,7 +1339,7 @@ let certTypeBytes ct =
 (** Parsing function for the certificate type *)
 val parseCertType: pinverse_t certTypeBytes
 let parseCertType b =
-  match cbyte b with
+  match b.[0ul] with
   | 1z -> Correct RSA_sign
   | 2z -> Correct DSA_sign
   | 3z -> Correct RSA_fixed_dh
@@ -1355,7 +1356,7 @@ let inverse_certType x = ()
 
 val pinverse_certType: x:_ -> Lemma
   (requires True)
-  (ensures (lemma_pinverse_f_g Seq.equal certTypeBytes parseCertType x))
+  (ensures (lemma_pinverse_f_g Bytes.equal certTypeBytes parseCertType x))
   [SMTPat (certTypeBytes (Correct?._0 (parseCertType x)))]
 let pinverse_certType x = ()
 
@@ -1376,7 +1377,7 @@ val parseCertificateTypeList: data:bytes -> Tot (list certType) (decreases (leng
 let rec parseCertificateTypeList data =
   if length data = 0 then []
   else
-    let (thisByte,data) = FStar.Bytes.split data 1 in
+    let (thisByte,data) = split data 1ul in
     match parseCertType thisByte with
     | Error z -> // we skip this one
       parseCertificateTypeList data
@@ -1409,7 +1410,7 @@ let defaultCertTypes sign cs =
 
 
 (** Type definition of the Distinguished Name of a certificate *)
-type dn = s:string{length(utf8 s) < 256}
+type dn = s:string{length(utf8_encode s) < 256}
 
 (** Serializing function for a list of Distinguished Names of certificates *)
 val distinguishedNameListBytes: names:list dn -> Tot (b:bytes{length b <= op_Multiply 258 (List.Tot.length names)})
@@ -1417,8 +1418,8 @@ let rec distinguishedNameListBytes names =
   match names with
   | [] -> empty_bytes
   | h::t ->
-    lemma_repr_bytes_values (length (utf8 h));
-    let name = vlbytes 2 (utf8 h) in
+    lemma_repr_bytes_values (length (utf8_encode h));
+    let name = vlbytes 2 (utf8_encode h) in
     name @| distinguishedNameListBytes t
 
 (** Parsing function for a list of Distinguished Names of certificates *)
@@ -1437,7 +1438,7 @@ let rec parseDistinguishedNameList data res =
 	match iutf8_opt nameBytes with
         | None -> Error(AD_decode_error, perror __SOURCE_FILE__ __LINE__ "")
         | Some name ->
-	  if length (utf8 name) < 256 then
+	  if length (utf8_encode name) < 256 then
           let res = name :: res in
           parseDistinguishedNameList data res
 	  else Error(AD_decode_error, perror __SOURCE_FILE__ __LINE__ "")
@@ -1488,7 +1489,7 @@ let inverse_configurationId x =
 
 val pinverse_configurationId: x:_ -> Lemma
   (requires True)
-  (ensures (lemma_pinverse_f_g Seq.equal configurationIdBytes parseConfigurationId x))
+  (ensures (lemma_pinverse_f_g Bytes.equal configurationIdBytes parseConfigurationId x))
   [SMTPat (configurationIdBytes (Correct?._0 (parseConfigurationId x)))]
 let pinverse_configurationId x = ()
 
@@ -1510,7 +1511,7 @@ let earlyDataTypeBytes edt =
 (** Parsing function for Early Data values *)
 val parseEarlyDataType: pinverse_t earlyDataTypeBytes
 let parseEarlyDataType b =
-  match cbyte b with
+  match b.[0ul] with
   | 1z -> Correct ClientAuthentication
   | 2z -> Correct EarlyData
   | 3z -> Correct ClientAuthenticationAndData
@@ -1526,7 +1527,7 @@ let inverse_earlyDataType x = ()
 
 val pinverse_earlyDataType: x:_ -> Lemma
   (requires True)
-  (ensures (lemma_pinverse_f_g Seq.equal earlyDataTypeBytes parseEarlyDataType x))
+  (ensures (lemma_pinverse_f_g Bytes.equal earlyDataTypeBytes parseEarlyDataType x))
   [SMTPat (earlyDataTypeBytes (Correct?._0 (parseEarlyDataType x)))]
 let pinverse_earlyDataType x = ()
 
@@ -1548,7 +1549,7 @@ let configurationExtensionBytes ce =
 val parseConfigurationExtension: pinverse_t configurationExtensionBytes
 let parseConfigurationExtension b =
   if length b >= 4 then
-    let (typ,payload) = split b 2 in
+    let (typ,payload) = split b 2ul in
     match vlparse 2 payload with
     | Correct payload -> Correct (UnknownConfigurationExtension typ payload)
     | Error z -> Error z
@@ -1564,16 +1565,16 @@ let inverse_configurationExtension x =
   match x with
   | UnknownConfigurationExtension typ payload ->
   let b = typ @| vlbytes 2 payload in
-  let b0,b1 = split b 2 in
-  let vl,b = split b1 2 in
+  let b0,b1 = split b 2ul in
+  let vl,b = split b1 2ul in
   vlparse_vlbytes 2 b;
-  assert (Seq.equal vl (bytes_of_int 2 (length b)));
-  assert (Seq.equal b0 typ);
-  assert (Seq.equal b payload)
+  assert (Bytes.equal vl (bytes_of_int 2 (length b)));
+  assert (Bytes.equal b0 typ);
+  assert (Bytes.equal b payload)
 
 val pinverse_configurationExtension: x:_ -> Lemma
   (requires True)
-  (ensures (lemma_pinverse_f_g Seq.equal configurationExtensionBytes parseConfigurationExtension x))
+  (ensures (lemma_pinverse_f_g Bytes.equal configurationExtensionBytes parseConfigurationExtension x))
   [SMTPat (configurationExtensionBytes (Correct?._0 (parseConfigurationExtension x)))]
 let pinverse_configurationExtension x = ()
 
@@ -1601,10 +1602,11 @@ let parseConfigurationExtensions b =
     fun b exts ->
     if length b > 0 then
       if length b >= 4 then
-	let typ, len, data = split2 b 2 2 in
+	let typ, len_data = split b 2ul in
+        let len, data = split len_data 2ul in
 	let len = int_of_bytes len in
 	if length b >= 4 + len then
-	  let ext, bytes = split b len in
+	  let ext, bytes = split_ b len in
 	  match parseConfigurationExtension ext with
 	  | Correct(ext') -> aux bytes (ext'::exts)
 	  | Error(z) -> Error(z)
@@ -1644,7 +1646,7 @@ let rec signatureSchemeListBytes_aux_is_injective
   (b2: bytes { length b1 == length b2 } )
   (algs2': list signatureScheme{ length b2 + op_Multiply 2 (List.Tot.length algs2') == op_Multiply 2 (List.Tot.length algs2) })
 : Lemma
-  (requires (Seq.equal (signatureSchemeListBytes_aux algs1 b1 algs1') (signatureSchemeListBytes_aux algs2 b2 algs2')))
+  (requires (Bytes.equal (signatureSchemeListBytes_aux algs1 b1 algs1') (signatureSchemeListBytes_aux algs2 b2 algs2')))
   (ensures (b1 == b2 /\ algs1' == algs2'))
   (decreases algs1')
 = match algs1', algs2' with
@@ -1653,7 +1655,7 @@ let rec signatureSchemeListBytes_aux_is_injective
     let shb1 = signatureSchemeBytes alg1 in
     let shb2 = signatureSchemeBytes alg2 in
     signatureSchemeListBytes_aux_is_injective algs1 (shb1 @| b1) algs1_ algs2 (shb2 @| b2) algs2_;
-    lemma_append_inj shb1 b1 shb2 b2;
+    //lemma_append_inj shb1 b1 shb2 b2; //TODO bytes NS 09/27
     signatureSchemeBytes_is_injective alg1 alg2
 
 val signatureSchemeListBytes: algs:signatureSchemeList
@@ -1669,7 +1671,7 @@ let signatureSchemeListBytes_is_injective
   (algs2: signatureSchemeList)
   (s2: bytes)
 : Lemma
-  (requires (Seq.equal (signatureSchemeListBytes algs1 @| s1) (signatureSchemeListBytes algs2 @| s2)))
+  (requires (Bytes.equal (signatureSchemeListBytes algs1 @| s1) (signatureSchemeListBytes algs2 @| s2)))
   (ensures (algs1 == algs2 /\ s1 == s2))
 = let pl1 = signatureSchemeListBytes_aux algs1 empty_bytes algs1 in
   lemma_repr_bytes_values (length pl1);
@@ -1689,7 +1691,7 @@ let parseSignatureSchemeList b =
       (decreases (length b')) = fun algs b' ->
     if length b' > 0 then
       if length b' >= 2 then
-      let alg, bytes = split b' 2 in
+      let alg, bytes = split b' 2ul in
       match parseSignatureScheme alg with
       | Correct sha -> aux (sha::algs) bytes
       | Error z     -> Error z
