src/tls/Curve25519.fst
@@ -11,6 +11,7 @@ open Platform.Error
 
 module X = Spec.Curve25519
 module CC = CoreCrypto
+module U32 = FStar.UInt32
 
 type scalar = lbytes 32
 type point = lbytes 32
@@ -23,13 +24,11 @@ let rand: ref (n:nat -> ST (lbytes n) (requires fun h->True) (ensures fun h0 _ h
   ralloc root CC.random
 
 // FIXME: Convert between Platform bytes (Seq.seq Char.char) and Hacl.Spec.Lib.bytes (Seq.seq UInt8.t)
-let bytes2hacl (b:bytes) : Tot (s:Seq.seq UInt8.t{Seq.length s = Seq.length b}) =
-  Seq.init (length b) (fun i ->
-    UInt8.uint_to_t (FStar.Char.int_of_char (FStar.Bytes.index b i)))
+let bytes2hacl (b:bytes) : Tot (s:Seq.seq UInt8.t{Seq.length s = length b}) =
+  Seq.init (length b) (fun i -> FStar.Bytes.get b (U32.uint_to_t i))
 
 let hacl2bytes (s:Seq.seq UInt8.t) : Tot (b:bytes{length b = Seq.length s}) =
-  FStar.Bytes.initBytes (Seq.length s) (fun i ->
-    FStar.Char.char_of_int (UInt8.v (Seq.index s i)))
+  FStar.Bytes.init (FStar.UInt32.uint_to_t (Seq.length s)) (fun i -> Seq.index s (U32.v i))
 
 let point_of_scalar (s:scalar) : Tot point =
   let base_point = Seq.upd (Seq.create 32 0uy) 0 9uy in
